src/Program_Model/VIMP/VIMP_Source_Print.thy
@@ -11,14 +11,14 @@ text \<open>
   depends on it.
 \<close>
 
-fun string_of_nat :: "nat \<Rightarrow> string" where
+fun string_of_nat :: "nat \<Rightarrow> String.literal" where
   "string_of_nat n =
-     (if n < 10 then [char_of (n + 48)]
-      else string_of_nat (n div 10) @ [char_of (n mod 10 + 48)])"
+     (if n < 10 then String.implode [char_of (n + 48)]
+      else string_of_nat (n div 10) + String.implode [char_of (n mod 10 + 48)])"
 
-definition string_of_int :: "int \<Rightarrow> string" where
+definition string_of_int :: "int \<Rightarrow> String.literal" where
   "string_of_int i =
-     (if i < 0 then ''-'' @ string_of_nat (nat (- i))
+     (if i < 0 then STR ''-'' + string_of_nat (nat (- i))
       else string_of_nat (nat i))"
 
 text \<open>\<open>exp_prio\<close> mirrors the grammar's mixfix priorities level for level, so
@@ -45,116 +45,147 @@ fun exp_prio :: "exp \<Rightarrow> nat" where
 | "exp_prio (And _ _) = 40"
 | "exp_prio (Or _ _) = 30"
 
-fun string_of_exp :: "nat \<Rightarrow> exp \<Rightarrow> string" where
+fun string_of_exp :: "nat \<Rightarrow> exp \<Rightarrow> String.literal" where
   "string_of_exp min_prio e =
      (let body =
         (case e of
            N n \<Rightarrow> string_of_int n
-         | V x \<Rightarrow> String.explode x
-         | Plus a b \<Rightarrow> string_of_exp 70 a @ ''+'' @ string_of_exp 71 b
-         | Minus a b \<Rightarrow> string_of_exp 70 a @ ''-'' @ string_of_exp 71 b
-         | Times a b \<Rightarrow> string_of_exp 80 a @ ''*'' @ string_of_exp 81 b
-         | Div a b \<Rightarrow> string_of_exp 80 a @ ''/'' @ string_of_exp 81 b
-         | Mod a b \<Rightarrow> string_of_exp 80 a @ ''%'' @ string_of_exp 81 b
-         | Less a b \<Rightarrow> string_of_exp 61 a @ ''<'' @ string_of_exp 61 b
-         | LessEq a b \<Rightarrow> string_of_exp 61 a @ ''<='' @ string_of_exp 61 b
-         | Greater a b \<Rightarrow> string_of_exp 61 a @ ''>'' @ string_of_exp 61 b
-         | GreaterEq a b \<Rightarrow> string_of_exp 61 a @ ''>='' @ string_of_exp 61 b
-         | NotEq a b \<Rightarrow> string_of_exp 51 a @ ''!='' @ string_of_exp 51 b
-         | Eq a b \<Rightarrow> string_of_exp 51 a @ ''=='' @ string_of_exp 51 b
-         | Not a \<Rightarrow> ''!'' @ string_of_exp 90 a
-         | And a b \<Rightarrow> string_of_exp 40 a @ ''&&'' @ string_of_exp 41 b
-         | Or a b \<Rightarrow> string_of_exp 30 a @ ''||'' @ string_of_exp 31 b)
-      in if exp_prio e < min_prio then ''('' @ body @ '')'' else body)"
+         | V x \<Rightarrow> x
+         | Plus a b \<Rightarrow> string_of_exp 70 a + STR ''+'' + string_of_exp 71 b
+         | Minus a b \<Rightarrow> string_of_exp 70 a + STR ''-'' + string_of_exp 71 b
+         | Times a b \<Rightarrow> string_of_exp 80 a + STR ''*'' + string_of_exp 81 b
+         | Div a b \<Rightarrow> string_of_exp 80 a + STR ''/'' + string_of_exp 81 b
+         | Mod a b \<Rightarrow> string_of_exp 80 a + STR ''%'' + string_of_exp 81 b
+         | Less a b \<Rightarrow> string_of_exp 61 a + STR ''<'' + string_of_exp 61 b
+         | LessEq a b \<Rightarrow> string_of_exp 61 a + STR ''<='' + string_of_exp 61 b
+         | Greater a b \<Rightarrow> string_of_exp 61 a + STR ''>'' + string_of_exp 61 b
+         | GreaterEq a b \<Rightarrow> string_of_exp 61 a + STR ''>='' + string_of_exp 61 b
+         | NotEq a b \<Rightarrow> string_of_exp 51 a + STR ''!='' + string_of_exp 51 b
+         | Eq a b \<Rightarrow> string_of_exp 51 a + STR ''=='' + string_of_exp 51 b
+         | Not a \<Rightarrow> STR ''!'' + string_of_exp 90 a
+         | And a b \<Rightarrow> string_of_exp 40 a + STR ''&&'' + string_of_exp 41 b
+         | Or a b \<Rightarrow> string_of_exp 30 a + STR ''||'' + string_of_exp 31 b)
+      in if exp_prio e < min_prio then STR ''('' + body + STR '')'' else body)"
 
 lemma string_of_exp_comparison_precedence:
-  "string_of_exp 0 (Eq (N 2) (Less (N 3) (N 4))) = ''2==3<4''"
-  "string_of_exp 0 (Less (Eq (N 2) (N 3)) (N 4)) = ''(2==3)<4''"
-  "string_of_exp 0 (NotEq (GreaterEq (N 2) (N 3)) (N 0)) = ''2>=3!=0''"
-  "string_of_exp 0 (GreaterEq (N 2) (NotEq (N 3) (N 0))) = ''2>=(3!=0)''"
+  "string_of_exp 0 (Eq (N 2) (Less (N 3) (N 4))) = STR ''2==3<4''"
+  "string_of_exp 0 (Less (Eq (N 2) (N 3)) (N 4)) = STR ''(2==3)<4''"
+  "string_of_exp 0 (NotEq (GreaterEq (N 2) (N 3)) (N 0)) = STR ''2>=3!=0''"
+  "string_of_exp 0 (GreaterEq (N 2) (NotEq (N 3) (N 0))) = STR ''2>=(3!=0)''"
   by eval+
 
-definition source_nl :: string where "source_nl = [CHR 0x0A]"
+definition source_nl :: String.literal where
+  "source_nl = String.implode [CHR 0x0A]"
 
-fun join_source :: "string \<Rightarrow> string list \<Rightarrow> string" where
-  "join_source sep [] = []"
+fun join_source :: "String.literal \<Rightarrow> String.literal list \<Rightarrow> String.literal" where
+  "join_source sep [] = STR ''''"
 | "join_source sep [s] = s"
-| "join_source sep (s # ss) = s @ sep @ join_source sep ss"
+| "join_source sep (s # ss) = s + sep + join_source sep ss"
 
-fun string_of_com :: "com \<Rightarrow> string" where
-  "string_of_com SKIP = ''skip;''"
-| "string_of_com (Assign x e) = String.explode x @ '' = '' @ string_of_exp 0 e @ '';''"
-| "string_of_com (VIMP_Proc.com.Check c) = ''__voblint_check('' @ string_of_exp 0 c @ '');''"
+fun string_of_com :: "com \<Rightarrow> String.literal" where
+  "string_of_com SKIP = STR ''skip;''"
+| "string_of_com (Assign x e) =
+    x + STR '' = '' + string_of_exp 0 e + STR '';''"
+| "string_of_com (VIMP_Proc.com.Check c) =
+    STR ''__voblint_check('' + string_of_exp 0 c + STR '');''"
 | "string_of_com (Seq c1 c2) =
-    string_of_com c1 @ source_nl @ string_of_com c2"
+    string_of_com c1 + source_nl + string_of_com c2"
 | "string_of_com (If b c1 c2) =
-    ''if ('' @ string_of_exp 0 b @ '') { '' @ string_of_com c1
-    @ (if c2 = SKIP then '' }'' else '' } else { '' @ string_of_com c2 @ '' }'')"
+    STR ''if ('' + string_of_exp 0 b + STR '') { '' + string_of_com c1
+    + (if c2 = SKIP
+       then STR '' }''
+       else STR '' } else { '' + string_of_com c2 + STR '' }'')"
 | "string_of_com (While b c) =
-    ''while ('' @ string_of_exp 0 b @ '') { '' @ string_of_com c @ '' }''"
+    STR ''while ('' + string_of_exp 0 b + STR '') { ''
+      + string_of_com c + STR '' }''"
 | "string_of_com (Call dst p es) =
     (case dst of
-      None \<Rightarrow> String.explode p @ ''('' @ join_source '', '' (map (string_of_exp 0) es) @ '');''
-    | Some x \<Rightarrow> String.explode x @ '' = '' @ String.explode p @ ''(''
-        @ join_source '', '' (map (string_of_exp 0) es) @ '');'')"
-| "string_of_com (Return (Some e)) = ''return '' @ string_of_exp 0 e @ '';''"
-| "string_of_com (Return None) = ''return;''"
-| "string_of_com Restore = ''restore''"
-| "string_of_com Unwind = ''<unwind>''"
+       None \<Rightarrow>
+         p + STR ''(''
+           + join_source (STR '', '') (map (string_of_exp 0) es)
+           + STR '');''
+     | Some x \<Rightarrow>
+         x + STR '' = '' + p + STR ''(''
+           + join_source (STR '', '') (map (string_of_exp 0) es)
+           + STR '');'')"
+| "string_of_com (Return (Some e)) =
+    STR ''return '' + string_of_exp 0 e + STR '';''"
+| "string_of_com (Return None) = STR ''return;''"
+| "string_of_com Restore = STR ''restore''"
+| "string_of_com Unwind = STR ''<unwind>''"
 
-fun source_indent :: "nat \<Rightarrow> string" where
-  "source_indent 0 = []"
-| "source_indent (Suc n) = ''  '' @ source_indent n"
+fun source_indent :: "nat \<Rightarrow> String.literal" where
+  "source_indent 0 = STR ''''"
+| "source_indent (Suc n) = STR ''  '' + source_indent n"
 
 text \<open>Append a suffix to the last line of a rendered fragment.\<close>
-fun append_last :: "string \<Rightarrow> string list \<Rightarrow> string list" where
+
+fun append_last ::
+  "String.literal \<Rightarrow> String.literal list \<Rightarrow> String.literal list" where
   "append_last suffix [] = []"
-| "append_last suffix [s] = [s @ suffix]"
+| "append_last suffix [s] = [s + suffix]"
 | "append_last suffix (s # ss) = s # append_last suffix ss"
 
-fun pretty_source_lines_com :: "nat \<Rightarrow> com \<Rightarrow> string list" where
-  "pretty_source_lines_com n SKIP = [source_indent n @ ''skip;'']"
+fun pretty_source_lines_com ::
+  "nat \<Rightarrow> com \<Rightarrow> String.literal list" where
+  "pretty_source_lines_com n SKIP =
+    [source_indent n + STR ''skip;'']"
 | "pretty_source_lines_com n (Assign x e) =
-    [source_indent n @ String.explode x @ '' = '' @ string_of_exp 0 e @ '';'']"
+    [source_indent n + x + STR '' = '' + string_of_exp 0 e + STR '';'']"
 | "pretty_source_lines_com n (VIMP_Proc.com.Check c) =
-    [source_indent n @ ''__voblint_check('' @ string_of_exp 0 c @ '');'']"
+    [source_indent n + STR ''__voblint_check(''
+       + string_of_exp 0 c + STR '');'']"
 | "pretty_source_lines_com n (Seq c1 c2) =
     pretty_source_lines_com n c1 @ pretty_source_lines_com n c2"
 | "pretty_source_lines_com n (If b c1 c2) =
-    [source_indent n @ ''if ('' @ string_of_exp 0 b @ '') {'']
+    [source_indent n + STR ''if ('' + string_of_exp 0 b + STR '') {'']
     @ pretty_source_lines_com (n + 2) c1
-    @ (if c2 = SKIP then [] else
-        [source_indent n @ ''} else {''] @ pretty_source_lines_com (n + 2) c2)
-    @ [source_indent n @ ''}'']"
+    @ (if c2 = SKIP then []
+       else
+         [source_indent n + STR ''} else {'']
+         @ pretty_source_lines_com (n + 2) c2)
+    @ [source_indent n + STR ''}'']"
 | "pretty_source_lines_com n (While b c) =
-    [source_indent n @ ''while ('' @ string_of_exp 0 b @ '') {'']
+    [source_indent n + STR ''while ('' + string_of_exp 0 b + STR '') {'']
     @ pretty_source_lines_com (n + 2) c
-    @ [source_indent n @ ''}'']"
+    @ [source_indent n + STR ''}'']"
 | "pretty_source_lines_com n (Call dst p es) =
-    [source_indent n @ string_of_com (Call dst p es)]"
+    [source_indent n + string_of_com (Call dst p es)]"
 | "pretty_source_lines_com n (Return e) =
-    [source_indent n @ string_of_com (Return e)]"
-| "pretty_source_lines_com n Restore = [source_indent n @ ''restore'']"
-| "pretty_source_lines_com n Unwind = [source_indent n @ ''<unwind>'']"
+    [source_indent n + string_of_com (Return e)]"
+| "pretty_source_lines_com n Restore =
+    [source_indent n + STR ''restore'']"
+| "pretty_source_lines_com n Unwind =
+    [source_indent n + STR ''<unwind>'']"
 
-definition pretty_source_lines_proc :: "nat \<Rightarrow> pname \<Rightarrow> proc_decl \<Rightarrow> string list" where
+definition pretty_source_lines_proc ::
+  "nat \<Rightarrow> pname \<Rightarrow> proc_decl \<Rightarrow> String.literal list" where
   "pretty_source_lines_proc n p decl =
-    (source_indent n @ ''fun '' @ String.explode p @ ''(''
-       @ join_source '', '' (map String.explode (formals decl)) @ '') {'')
-    # pretty_source_lines_com (n + 2) (body decl)
-    @ [source_indent n @ ''}'']"
+    (source_indent n + STR ''fun '' + p + STR ''(''
+       + join_source (STR '', '') (formals decl) + STR '') {'')
+    # (pretty_source_lines_com (n + 2) (body decl)
+       @ [source_indent n + STR ''}''])"
 
 text \<open>Canonical concrete syntax: no \<open>program { ... }\<close> wrapper, and no
   \<open>global\<close> line when \<open>globals\<close> is empty.\<close>
+
 definition pretty_string_of_program ::
-  "proc_table \<Rightarrow> pname list \<Rightarrow> com \<Rightarrow> vname list \<Rightarrow> string" where
+  "proc_table \<Rightarrow> pname list \<Rightarrow> com \<Rightarrow> vname list \<Rightarrow> String.literal" where
   "pretty_string_of_program \<Pi> ps main globals =
     join_source source_nl
       ((if globals = [] then []
-        else [''global '' @ join_source '', '' (map String.explode globals) @ '';''])
-      @ concat (map (\<lambda>p. case \<Pi> p of
-          None \<Rightarrow> [''procedure '' @ String.explode p @ '' <missing>'']
-        | Some decl \<Rightarrow> pretty_source_lines_proc 0 p decl) ps)
-      @ [''fun main() {''] @ pretty_source_lines_com 2 main @ [''}''])"
+        else
+          [STR ''global ''
+             + join_source (STR '', '') globals
+             + STR '';''])
+       @ concat
+           (map
+             (\<lambda>p. case \<Pi> p of
+                None \<Rightarrow> [STR ''procedure '' + p + STR '' <missing>'']
+              | Some decl \<Rightarrow> pretty_source_lines_proc 0 p decl)
+             ps)
+       @ [STR ''fun main() {'']
+       @ pretty_source_lines_com 2 main
+       @ [STR ''}''])"
 
 end
