src/Executable_Surface/CLI/Analysis_Graph_Naming.thy
@@ -37,20 +37,20 @@ text \<open>
   frame is empty.
 \<close>
 
-definition cs_show_context :: "cfg_node list \<Rightarrow> string" where
-  "cs_show_context ctx = concat (map (\<lambda>u. string_of_cfg_node u @ '' '') ctx)"
+definition cs_show_context :: "cfg_node list \<Rightarrow> String.literal" where
+  "cs_show_context ctx = join_esc_nl (map (\<lambda>u. string_of_cfg_node u + STR '' '') ctx)"
 
 definition cs_context_key :: "cfg_node list \<Rightarrow> String.literal" where
-  "cs_context_key ctx = String.implode (cs_show_context ctx)"
+  "cs_context_key ctx = cs_show_context ctx"
 
 definition cs_graph_route ::
   "nat \<Rightarrow> pp \<Rightarrow> cfg_node list \<Rightarrow> call_action \<Rightarrow> 'd \<Rightarrow> cfg_node list option" where
   "cs_graph_route k u ctx ca d = Some (cs_route k u ctx d ca)"
 
-definition cs_cluster_label :: "string \<Rightarrow> cfg_node list \<Rightarrow> string" where
+definition cs_cluster_label :: "String.literal \<Rightarrow> cfg_node list \<Rightarrow> String.literal" where
   "cs_cluster_label owner ctx =
-     (if ctx = [] then owner @ '' / root context''
-      else owner @ '' / call-string='' @ cs_show_context ctx)"
+     (if ctx = [] then owner + STR '' / root context''
+      else owner + STR '' / call-string='' + cs_show_context ctx)"
 
 subsection \<open>Naming nodes and clusters\<close>
 
@@ -65,6 +65,7 @@ text \<open>
 definition entry_proc_exit :: "cfg \<Rightarrow> cfg_node" where
   "entry_proc_exit g =
     (case cfg_entry g of FunctionEntry p \<Rightarrow> FunctionResult p | p \<Rightarrow> p)"
+
 fun analysis_node_position :: "('ctx, 'g) analysis_node list
   \<Rightarrow> ('ctx, 'g) analysis_node \<Rightarrow> nat" where
   "analysis_node_position [] n = 0"
@@ -73,7 +74,7 @@ fun analysis_node_position :: "('ctx, 'g) analysis_node list
 
 fun owner_contexts ::
   "('ctx, 'g, 'a, 'd) analysis_graph_config \<Rightarrow> ('ctx, 'g) analysis_node list
-    \<Rightarrow> (string \<times> 'ctx) list" where
+    \<Rightarrow> (String.literal \<times> 'ctx) list" where
   "owner_contexts cfg [] = []"
 | "owner_contexts cfg (LocalNode p ctx # ns) =
     (owner_of cfg p, ctx) # owner_contexts cfg ns"
@@ -87,14 +88,18 @@ fun context_position :: "'a list \<Rightarrow> 'a \<Rightarrow> nat" where
 
 definition analysis_node_id ::
   "('ctx, 'g, 'a, 'd) analysis_graph_config \<Rightarrow> ('ctx, 'g) analysis_node list
-    \<Rightarrow> ('ctx, 'g) analysis_node \<Rightarrow> string" where
+    \<Rightarrow> ('ctx, 'g) analysis_node \<Rightarrow> String.literal" where
   "analysis_node_id cfg ns n =
     (case n of
-      LocalNode p ctx \<Rightarrow> owner_of cfg p @ ''_'' @ string_of_cfg_node p @ ''_ctx''
-        @ string_of_nat (context_position (remdups (owner_contexts cfg ns))
-            (owner_of cfg p, ctx))
-    | GlobalNode k \<Rightarrow> ''global_'' @ string_of_nat (analysis_node_position ns n)
-    | SourceNode src \<Rightarrow> ''source'')" 
+      LocalNode p ctx \<Rightarrow>
+        owner_of cfg p + STR ''_'' + string_of_cfg_node p + STR ''_ctx''
+          + string_of_nat
+              (context_position
+                (remdups (owner_contexts cfg ns))
+                (owner_of cfg p, ctx))
+    | GlobalNode k \<Rightarrow>
+        STR ''global_'' + string_of_nat (analysis_node_position ns n)
+    | SourceNode src \<Rightarrow> STR ''source'')"
 
 fun analysis_cluster_position :: "('ctx, 'g) analysis_cluster list
   \<Rightarrow> ('ctx, 'g) analysis_cluster \<Rightarrow> nat" where
@@ -104,13 +109,14 @@ fun analysis_cluster_position :: "('ctx, 'g) analysis_cluster list
      else Suc (analysis_cluster_position clusters cluster))"
 
 definition analysis_cluster_id :: "('ctx, 'g) analysis_cluster list
-  \<Rightarrow> ('ctx, 'g) analysis_cluster \<Rightarrow> string" where
+  \<Rightarrow> ('ctx, 'g) analysis_cluster \<Rightarrow> String.literal" where
   "analysis_cluster_id clusters cluster =
     (case cluster of
-      GlobalCluster \<Rightarrow> ''cluster_globals''
-    | SourceCluster \<Rightarrow> ''cluster_source''
-    | ContextCluster owner ctx \<Rightarrow> ''cluster_ctx_''
-        @ string_of_nat (analysis_cluster_position clusters cluster))"
+      GlobalCluster \<Rightarrow> STR ''cluster_globals''
+    | SourceCluster \<Rightarrow> STR ''cluster_source''
+    | ContextCluster owner ctx \<Rightarrow>
+        STR ''cluster_ctx_''
+          + string_of_nat (analysis_cluster_position clusters cluster))"
 
 definition analysis_nodes_in_cluster ::
   "('ctx, 'g, 'a, 'd) analysis_graph_config \<Rightarrow> ('ctx, 'g) analysis_cluster
@@ -123,43 +129,12 @@ definition analysis_nodes_in_cluster ::
       | (SourceCluster, SourceNode _) \<Rightarrow> True
       | _ \<Rightarrow> False) ns)"
 
-
-
-definition point_label :: "cfg \<Rightarrow> pp \<Rightarrow> string" where
+definition point_label :: "cfg \<Rightarrow> pp \<Rightarrow> String.literal" where
   "point_label g p =
     (case p of
-      FunctionEntry owner \<Rightarrow> ''entry_'' @ String.explode owner
-    | FunctionResult owner \<Rightarrow> ''exit_'' @ String.explode owner
+      FunctionEntry owner \<Rightarrow> STR ''entry_'' + owner
+    | FunctionResult owner \<Rightarrow> STR ''exit_'' + owner
     | Statement _ \<Rightarrow> string_of_cfg_node p)"
-
-text \<open>
-  The inverse of \<^const>\<open>join_esc_nl\<close>: splits a string joined with the literal
-  \<open>\n\<close> separator back into its original lines. A caller with multi-line
-  content to attach as one \<^typ>\<open>graph_node_annotation\<close> (a single flat
-  \<^const>\<open>annotation_label\<close> string, by design, so nothing here has to know
-  what an annotation means) already joins it with \<^const>\<open>join_esc_nl\<close> --- the
-  same convention the per-node label-line builder below uses. A renderer
-  consumes that joined form directly; the canonical snapshot needs the lines
-  apart again, hence this being used only there.
-
-  Characters are compared with \<open>=\<close> rather than pattern-matched against a
-  literal \<open>CHR\<close> value on a \<open>fun\<close> equation's left-hand side ---
-  \<open>HOL-Library.Code_Abstract_Char\<close> (pulled in for this session's OCaml code
-  generation) represents \<^typ>\<open>char\<close> abstractly for the code generator, which
-  then rejects a literal-\<open>CHR\<close> pattern as ``not a constructor''. An equality
-  test in the body has no such restriction.
-\<close>
-
-fun split_esc_nl_acc :: "string \<Rightarrow> string \<Rightarrow> string list" where
-  "split_esc_nl_acc acc [] = [rev acc]"
-| "split_esc_nl_acc acc [ch] = [rev (ch # acc)]"
-| "split_esc_nl_acc acc (ch1 # ch2 # rest) =
-    (if ch1 = CHR 0x5C \<and> ch2 = CHR 0x6E
-     then rev acc # split_esc_nl_acc [] rest
-     else split_esc_nl_acc (ch1 # acc) (ch2 # rest))"
-
-definition split_esc_nl :: "string \<Rightarrow> string list" where
-  "split_esc_nl s = split_esc_nl_acc [] s"
 
 text \<open>
   The per-node label as a line list, before \<^const>\<open>join_esc_nl\<close> escapes it
@@ -170,31 +145,39 @@ text \<open>
 
 definition contextual_node_label_lines ::
   "('ctx, 'g, 'a, 'd) analysis_graph_config \<Rightarrow> cfg
-    \<Rightarrow> (pp \<times> 'ctx + 'g \<Rightarrow> 'a) \<Rightarrow> ('ctx, 'g) analysis_node \<Rightarrow> string list" where
+    \<Rightarrow> (pp \<times> 'ctx + 'g \<Rightarrow> 'a) \<Rightarrow> ('ctx, 'g) analysis_node \<Rightarrow> String.literal list" where
   "contextual_node_label_lines cfg g sol n =
     (case n of
       LocalNode p ctx \<Rightarrow>
         point_label g p #
           show_local cfg p ctx (locals_for_pp cfg p)
             (local_of cfg (sol (Inl (p, ctx))))
-          @ (case return_slot_for_pp cfg p of None \<Rightarrow> []
-             | Some ret \<Rightarrow> format_return cfg p ctx ret
-                 (local_of cfg (sol (Inl (p, ctx)))))
-          @ (case node_annotation cfg p ctx of
+          @ (case return_slot_for_pp cfg p of
               None \<Rightarrow> []
-            | Some ann \<Rightarrow>
-                if annotation_label ann = '''' then [] else split_esc_nl (annotation_label ann))
+            | Some ret \<Rightarrow>
+                format_return cfg p ctx ret
+                  (local_of cfg (sol (Inl (p, ctx)))))
+          @ (case node_annotation cfg p ctx of
+               None \<Rightarrow> []
+             | Some ann \<Rightarrow> annotation_lines ann)
     | GlobalNode k \<Rightarrow>
-        show_global_key cfg k # show_global cfg k (globals_to_show cfg) (sol (Inr k))
+        show_global_key cfg k #
+          show_global cfg k (globals_to_show cfg) (sol (Inr k))
     | SourceNode src \<Rightarrow> [src])"
 
-
-definition source_action_label :: "cfg \<Rightarrow> edge_action \<Rightarrow> string" where
+definition source_action_label :: "cfg \<Rightarrow> edge_action \<Rightarrow> String.literal" where
   "source_action_label g a =
-    (case a of EA_Assign x e \<Rightarrow>
-       if x = ret_var then ''ret := '' @ string_of_exp 0 e else string_of_action a    | EA_Assume b \<Rightarrow> string_of_exp 0 b
-    | EA_AssumeNot b \<Rightarrow> ''not ('' @ string_of_exp 0 b @ '')''
-    | EA_Ret _ p \<Rightarrow> if cfg_entry g = FunctionEntry p then ''terminate'' else string_of_action a
+    (case a of
+      EA_Assign x e \<Rightarrow>
+        if x = ret_var
+        then STR ''ret := '' + string_of_exp 0 e
+        else string_of_action a
+    | EA_Assume b \<Rightarrow> string_of_exp 0 b
+    | EA_AssumeNot b \<Rightarrow> STR ''not ('' + string_of_exp 0 b + STR '')''
+    | EA_Ret _ p \<Rightarrow>
+        if cfg_entry g = FunctionEntry p
+        then STR ''terminate''
+        else string_of_action a
     | _ \<Rightarrow> string_of_action a)"
 
 text \<open>
@@ -202,27 +185,34 @@ text \<open>
   no presentation syntax, for the canonical regression snapshot below.
 \<close>
 
-definition canonical_edge_kind_text :: "cfg \<Rightarrow> analysis_edge_kind \<Rightarrow> string" where
+definition canonical_edge_kind_text ::
+  "cfg \<Rightarrow> analysis_edge_kind \<Rightarrow> String.literal" where
   "canonical_edge_kind_text g kind =
     (case kind of
       IntraEdge a \<Rightarrow> source_action_label g a
-    | EnterEdge callee a \<Rightarrow> ''enter '' @ callee @ ''(''
-        @ (case a of CallEdge _ _ es \<Rightarrow> join_source '', '' (map (string_of_exp 0) es)) @ '')''
-    | CombineEdge call dst ret \<Rightarrow> ''combine''
-        @ (case (dst, ret) of
-             (Some x, Some r) \<Rightarrow> '' '' @ String.explode x @ '' := '' @ String.explode r
-           | (Some x, None) \<Rightarrow> '' '' @ String.explode x
-           | (None, _) \<Rightarrow> '''')
-    | CallToReturnEdge callee \<Rightarrow> ''call-to-return '' @ String.explode callee
-    | GlobalReadEdge \<Rightarrow> ''read global''
-    | GlobalWriteEdge \<Rightarrow> ''write global'')"
+    | EnterEdge callee a \<Rightarrow>
+        STR ''enter '' + callee + STR ''(''
+          + (case a of
+               CallEdge _ _ es \<Rightarrow>
+                 join_source (STR '', '') (map (string_of_exp 0) es))
+          + STR '')''
+    | CombineEdge call dst ret \<Rightarrow>
+        STR ''combine''
+          + (case (dst, ret) of
+               (Some x, Some r) \<Rightarrow> STR '' '' + x + STR '' := '' + r
+             | (Some x, None) \<Rightarrow> STR '' '' + x
+             | (None, _) \<Rightarrow> STR '''')
+    | CallToReturnEdge callee \<Rightarrow> STR ''call-to-return '' + callee
+    | GlobalReadEdge \<Rightarrow> STR ''read global''
+    | GlobalWriteEdge \<Rightarrow> STR ''write global'')"
 
 definition analysis_cluster_label ::
-  "('ctx, 'g, 'a, 'd) analysis_graph_config \<Rightarrow> ('ctx, 'g) analysis_cluster \<Rightarrow> string" where
+  "('ctx, 'g, 'a, 'd) analysis_graph_config
+    \<Rightarrow> ('ctx, 'g) analysis_cluster \<Rightarrow> String.literal" where
   "analysis_cluster_label cfg cluster =
     (case cluster of
       ContextCluster owner ctx \<Rightarrow> cluster_label cfg owner ctx
-    | GlobalCluster \<Rightarrow> ''Shared globals''
-    | SourceCluster \<Rightarrow> ''Source'')"
+    | GlobalCluster \<Rightarrow> STR ''Shared globals''
+    | SourceCluster \<Rightarrow> STR ''Source'')"
 
 end
